EffectSSA/Syntax/Untyped/Lemmas.lean
@@ -40,4 +40,12 @@ theorem toList_inj : p.toList = q.toList ↔ p = q := by
 theorem toList_append : (p ++ q).toList = p.toList ++ q.toList := by
   induction p generalizing q <;> cases q <;> grind
 
+/-! ### foldlM -/
+
+@[simp, grind =] theorem foldlM_nil [Monad m] (f : α → Instruction τ → m α) (init : α) :
+    foldlM f init (@nil τ) = pure init := by rfl
+
+@[simp, grind =] theorem foldlM_cons [Monad m] (f : α → Instruction τ → m α) (init : α) :
+    foldlM f init (i ;> p) = f init i >>= fun a => foldlM f a p := by rfl
+
 end InstructionSeq
